Lectures 1 and 2

teaching/eutypes2018/code/state/Heap.fsti
@@ -8,7 +8,7 @@ module Heap
   val sel : #a:Type -> heap -> ref a -> GTot a
   val addr_of: #a:Type -> ref a -> GTot nat
 
-  let modifies (s:set nat) (h0 h1 : heap) : Type0 =
-  (forall (a:Type) (r:ref a).{:pattern (sel h1 r)}
-    (~(addr_of r `mem` s)) ==> sel h1 r == sel h0 r)
+  let modifies (s:set nat) (h0 h1 : heap) =
+    forall (a:Type) (r:ref a).{:pattern (sel h1 r)}
+        ~(addr_of r `mem` s) ==> sel h1 r == sel h0 r
 // END: heap_model
